NoRef.v
@@ -45,7 +45,8 @@ Inductive no_ref (ad : addr) : tm -> Prop :=
                                    no_ref ad <{acq t1 x t2              }>
   | noref_cr    : forall ad' t,    no_ref ad t  ->
                                    no_ref ad <{cr ad' t                 }>
-  | noref_wait  : forall ad',      no_ref ad <{wait ad'                 }>
+  | noref_wait  : forall t,        no_ref ad t  ->
+                                   no_ref ad <{wait t                   }>
   | noref_reacq : forall ad',      no_ref ad <{reacq ad'                }>
   | noref_spawn : forall t,        no_ref ad t ->
                                    no_ref ad <{spawn t                  }>
@@ -73,7 +74,7 @@ Local Ltac _noref tt :=
   | H : no_ref _   <{_ := _                }> |- _ => tt H
   | H : no_ref _   <{acq _ _ _             }> |- _ => tt H
   | H : no_ref _   <{cr _ _                }> |- _ => tt H
-  | H : no_ref _   <{wait _                }> |- _ => clear H
+  | H : no_ref _   <{wait _                }> |- _ => tt H
   | H : no_ref _   <{reacq _               }> |- _ => clear H
   | H : no_ref _   <{spawn _               }> |- _ => tt H
   end.
@@ -123,21 +124,13 @@ Lemma noref_subst : forall ad x tx t,
   no_ref ad <{[x := tx] t}>.
 Proof. 
   intros. induction t; invc_noref;
-  simpl in *; try destruct _str_eq_dec; auto using no_ref.
-Qed.
-
-Lemma noref_fw : forall ad ad' t,
-  no_ref ad t ->
-  no_ref ad (fw ad' t).
-Proof. 
-  intros. induction t; invc_noref; simpl; auto using no_ref.
+  simpl; repeat destruct _str_eq_dec; auto using no_ref.
 Qed.
 
 (* preservation ------------------------------------------------------------ *)
 
 Local Ltac solve_noref_preservation :=
-  intros; ind_tstep; repeat invc_noref;
-  auto using noref_subst, noref_fw, no_ref.
+  intros; ind_tstep; repeat invc_noref; auto using noref_subst, no_ref.
 
 Lemma noref_preservation_none : forall ad t1 t2,
   no_ref ad t1 ->
@@ -198,15 +191,15 @@ Lemma noref_preservation_wrel : forall ad t1 t2 ad',
   no_ref ad t2.
 Proof. solve_noref_preservation. Qed.
 
-Lemma noref_preservation_spawn : forall ad t1 t2 tid' t',
+Lemma noref_preservation_spawn : forall ad t1 t2 t',
   no_ref ad t1 ->
-  t1 --[e_spawn tid' t']--> t2 ->
+  t1 --[e_spawn t']--> t2 ->
   no_ref ad t2.
 Proof. solve_noref_preservation. Qed.
 
-Lemma noref_preservation_spawned : forall ad t1 t2 tid' t',
+Lemma noref_preservation_spawned : forall ad t1 t2 t',
   no_ref ad t1 ->
-  t1 --[e_spawn tid' t']--> t2 ->
+  t1 --[e_spawn t']--> t2 ->
   no_ref ad t'.
 Proof. solve_noref_preservation. Qed.
 
@@ -277,6 +270,10 @@ Local Lemma inv_norefs_cr : forall ad t,
   no_refs <{cr ad t}> -> no_refs t.
 Proof. solve_inv_norefs. Qed.
 
+Local Lemma inv_norefs_wait : forall t,
+  no_refs <{wait t}> -> no_refs t.
+Proof. solve_inv_norefs. Qed.
+
 Local Lemma inv_norefs_spawn : forall t,
   no_refs <{spawn t}> -> no_refs t.
 Proof. solve_inv_norefs. Qed.
@@ -300,7 +297,7 @@ Ltac invc_norefs :=
   | H : no_refs <{_ := _      }> |- _ => eapply inv_norefs_asg   in H
   | H : no_refs <{acq _ _ _   }> |- _ => eapply inv_norefs_acq   in H
   | H : no_refs <{cr _ _      }> |- _ => eapply inv_norefs_cr    in H
-  | H : no_refs <{wait _      }> |- _ => clear H
+  | H : no_refs <{wait _      }> |- _ => eapply inv_norefs_wait  in H
   | H : no_refs <{reacq _     }> |- _ => clear H
   | H : no_refs <{spawn _     }> |- _ => eapply inv_norefs_spawn in H
   end;
