ValidWaits.v
@@ -1,319 +1,66 @@
 From Elo Require Import Core.
 
-(* ------------------------------------------------------------------------- *)
-(* no-waits                                                                  *)
-(* ------------------------------------------------------------------------- *)
-
-Inductive no_waits : tm -> Prop :=
-  | nowaits_unit   :                  no_waits <{unit                     }>
-  | nowaits_nat    : forall n,        no_waits <{nat n                    }>
-  | nowaits_plus   : forall t1 t2,    no_waits t1 ->
-                                      no_waits t2 ->
-                                      no_waits <{t1 + t2                  }>
-  | nowaits_monus  : forall t1 t2,    no_waits t1 ->
-                                      no_waits t2 ->
-                                      no_waits <{t1 - t2                  }>
-  | nowaits_seq    : forall t1 t2,    no_waits t1 ->
-                                      no_waits t2 ->
-                                      no_waits <{t1; t2                   }>
-  | nowaits_if     : forall t1 t2 t3, no_waits t1 ->
-                                      no_waits t2 ->
-                                      no_waits t3 ->
-                                      no_waits <{if t1 then t2 else t3 end}>
-  | nowaits_while  : forall t1 t2,    no_waits t1 ->
-                                      no_waits t2 ->
-                                      no_waits <{while t1 do t2 end}>
-  | nowaits_var    : forall x,        no_waits <{var x                    }>
-  | nowaits_fun    : forall x Tx t,   no_waits t           ->
-                                      no_waits <{fn x Tx t                }>
-  | nowaits_call   : forall t1 t2,    no_waits t1 ->
-                                      no_waits t2 ->
-                                      no_waits <{call t1 t2               }>
-  | nowaits_ref    : forall ad T,     no_waits <{&ad : T                  }>
-  | nowaits_new    : forall t T,      no_waits t  ->
-                                      no_waits <{new t : T                }>
-  | nowaits_init   : forall ad t T,   no_waits t  ->
-                                      no_waits <{init ad t : T            }>
-  | nowaits_load   : forall t,        no_waits t  ->
-                                      no_waits <{*t                       }>
-  | nowaits_asg    : forall t1 t2,    no_waits t1 ->
-                                      no_waits t2 ->
-                                      no_waits <{t1 := t2                 }>
-  | nowaits_acq    : forall t1 x t2,  no_waits t1 ->
-                                      no_waits t2 ->
-                                      no_waits <{acq t1 x t2              }>
-  | nowaits_cr     : forall ad t,     no_waits  t ->
-                                      no_waits <{cr ad t                  }>
-  | nowaits_reacq  : forall ad,       no_waits <{reacq ad                 }>
-  | nowaits_spawn  : forall t,        no_waits t  ->
-                                      no_waits <{spawn t                  }>
-  .
-
-Local Ltac _nowaits tt :=
-  match goal with
-  | H : no_waits <{unit                  }> |- _ => clear H
-  | H : no_waits <{nat _                 }> |- _ => clear H
-  | H : no_waits <{_ + _                 }> |- _ => tt H
-  | H : no_waits <{_ - _                 }> |- _ => tt H
-  | H : no_waits <{_; _                  }> |- _ => tt H
-  | H : no_waits <{if _ then _ else _ end}> |- _ => tt H
-  | H : no_waits <{while _ do _ end      }> |- _ => tt H
-  | H : no_waits <{var _                 }> |- _ => tt H
-  | H : no_waits <{fn _ _ _              }> |- _ => tt H
-  | H : no_waits <{call _ _              }> |- _ => tt H
-  | H : no_waits <{&_ : _                }> |- _ => clear H
-  | H : no_waits <{new _ : _             }> |- _ => tt H
-  | H : no_waits <{init _ _ : _          }> |- _ => tt H
-  | H : no_waits <{* _                   }> |- _ => tt H
-  | H : no_waits <{_ := _                }> |- _ => tt H
-  | H : no_waits <{acq _ _ _             }> |- _ => tt H
-  | H : no_waits <{cr _ _                }> |- _ => tt H
-  | H : no_waits <{wait _                }> |- _ => invc H
-  | H : no_waits <{reacq _               }> |- _ => clear H
-  | H : no_waits <{spawn _               }> |- _ => tt H
-  end.
-
-Ltac inv_nowaits  := _nowaits inv.
-Ltac invc_nowaits := _nowaits invc.
-
-(* preservation lemmas ----------------------------------------------------- *)
-
-Lemma nowaits_subst : forall t tx x,
-  no_waits t  ->
-  no_waits tx ->
-  no_waits <{[x := tx] t}>.
-Proof.
-  intros. induction t; invc_nowaits; simpl; try destruct _str_eq_dec;
-  auto using no_waits.
-Qed.
-
-(* ------------------------------------------------------------------------- *)
-(* matching-waits                                                            *)
-(* ------------------------------------------------------------------------- *)
-
-Inductive matching_waits (ad : addr) : tm -> Prop :=
-  | mwaits_unit   :                  matching_waits ad <{unit              }>
-  | mwaits_nat    : forall n,        matching_waits ad <{nat n             }>
-  | mwaits_plus   : forall t1 t2,    matching_waits ad t1 ->
-                                     matching_waits ad t2 ->
-                                     matching_waits ad <{t1 + t2           }>
-  | mwaits_monus  : forall t1 t2,    matching_waits ad t1 ->
-                                     matching_waits ad t2 ->
-                                     matching_waits ad <{t1 - t2           }>
-  | mwaits_seq    : forall t1 t2,    matching_waits ad t1 ->
-                                     matching_waits ad t2 ->
-                                     matching_waits ad <{t1; t2            }>
-  | mwaits_if     : forall t1 t2 t3, matching_waits ad t1 ->
-                                     matching_waits ad t2 ->
-                                     matching_waits ad t3 ->
-                                     matching_waits ad (tm_if t1 t2 t3)
-  | mwaits_while  : forall t1 t2,    matching_waits ad t1 ->
-                                     matching_waits ad t2 ->
-                                     matching_waits ad <{while t1 do t2 end}>
-  | mwaits_var    : forall x,        matching_waits ad <{var x             }>
-  | mwaits_fun    : forall x Tx t,   no_waits t           ->
-                                     matching_waits ad <{fn x Tx t         }>
-  | mwaits_call   : forall t1 t2,    matching_waits ad t1 ->
-                                     matching_waits ad t2 ->
-                                     matching_waits ad <{call t1 t2        }>
-  | mwaits_ref    : forall ad' T,    matching_waits ad <{&ad' : T          }>
-  | mwaits_new    : forall t T,      matching_waits ad t  ->
-                                     matching_waits ad <{new t : T         }>
-  | mwaits_init   : forall ad' t T,  matching_waits ad t  ->
-                                     matching_waits ad <{init ad' t : T    }>
-  | mwaits_load   : forall t,        matching_waits ad t  ->
-                                     matching_waits ad <{*t                }>
-  | mwaits_asg    : forall t1 t2,    matching_waits ad t1 ->
-                                     matching_waits ad t2 ->
-                                     matching_waits ad <{t1 := t2          }>
-  | mwaits_acq    : forall t1 x t2,  matching_waits ad t1 ->
-                                     matching_waits ad <{acq t1 x t2       }>
-  | mwaits_cr     : forall ad' t,    matching_waits ad' t ->
-                                     matching_waits ad <{cr ad' t          }>
-  | mwaits_wait   :                  matching_waits ad <{wait ad           }>
-  | mwaits_reacq  : forall ad',      matching_waits ad <{reacq ad'         }>
-  | mwaits_spawn  : forall t,        matching_waits ad t  ->
-                                     matching_waits ad <{spawn t           }>
-  .
-
-(* inversion --------------------------------------------------------------- *)
-
-Local Ltac _mwaits tt :=
-  match goal with
-  | H : matching_waits _ <{unit                  }> |- _ => clear H
-  | H : matching_waits _ <{nat _                 }> |- _ => clear H
-  | H : matching_waits _ <{_ + _                 }> |- _ => tt H
-  | H : matching_waits _ <{_ - _                 }> |- _ => tt H
-  | H : matching_waits _ <{_; _                  }> |- _ => tt H
-  | H : matching_waits _ <{if _ then _ else _ end}> |- _ => tt H
-  | H : matching_waits _ <{while _ do _ end      }> |- _ => tt H
-  | H : matching_waits _ <{var _                 }> |- _ => tt H
-  | H : matching_waits _ <{fn _ _ _              }> |- _ => tt H
-  | H : matching_waits _ <{call _ _              }> |- _ => tt H
-  | H : matching_waits _ <{&_ : _                }> |- _ => clear H
-  | H : matching_waits _ <{new _ : _             }> |- _ => tt H
-  | H : matching_waits _ <{init _ _ : _          }> |- _ => tt H
-  | H : matching_waits _ <{* _                   }> |- _ => tt H
-  | H : matching_waits _ <{_ := _                }> |- _ => tt H
-  | H : matching_waits _ <{acq _ _ _             }> |- _ => tt H
-  | H : matching_waits _ <{cr _ _                }> |- _ => tt H
-  | H : matching_waits _ <{wait _                }> |- _ => tt H
-  | H : matching_waits _ <{reacq _               }> |- _ => clear H
-  | H : matching_waits _ <{spawn _               }> |- _ => tt H
-  end.
-
-Ltac inv_mwaits  := _mwaits inv.
-Ltac invc_mwaits := _mwaits invc.
-
-(* lemmas ------------------------------------------------------------------ *)
-
-Lemma mwaits_from_nowaits : forall ad t,
-  no_waits t ->
-  matching_waits ad t.
-Proof.
-  intros. gendep ad.
-  induction t; intros; invc_nowaits; auto using matching_waits.
-Qed.
-
-Lemma nowaits_from_value1 : forall ad t,
-  matching_waits ad t ->
-  (* --- *)
-  value t ->
-  no_waits t.
-Proof.
-  intros * ? Hval. invc Hval; auto using no_waits.
-  invc_mwaits. auto using no_waits.
-Qed.
-
-(* preservation lemmas ----------------------------------------------------- *)
-
-Lemma mwaits_subst : forall ad t tx x,
-  value tx ->
-  (* --- *)
-  no_waits t ->
-  matching_waits ad tx ->
-  matching_waits ad <{[x := tx] t}>.
-Proof.
-  intros. eauto using mwaits_from_nowaits, nowaits_from_value1, nowaits_subst. 
-Qed.
-
-Lemma mwaits_fw : forall ad t,
-  matching_waits ad (fw ad t).
-Proof.
-  intros. gendep ad. induction t; intros; simpl; auto using matching_waits.
-  - constructor. admit.
-  - repeat spec. constructor. admit.
-Abort.
-
-(* preservation ------------------------------------------------------------ *)
-
-Local Ltac solve_mwaits_preservation :=
-  intros ad **; gendep ad;
-  ind_tstep; intros; repeat invc_mwaits; repeat constructor;
-  auto using mwaits_from_nowaits, mwaits_subst.
-
-Lemma mwaits_preservation_none : forall ad t1 t2,
-  matching_waits ad t1 ->
-  t1 --[e_none]--> t2 ->
-  matching_waits ad t2.
-Proof. solve_mwaits_preservation. Qed.
-
-Lemma mwaits_preservation_alloc : forall ad t1 t2 ad' T',
-  matching_waits ad t1 ->
-  t1 --[e_alloc ad' T']--> t2 ->
-  matching_waits ad t2.
-Proof. solve_mwaits_preservation. Qed.
-
-Lemma mwaits_preservation_init : forall ad t1 t2 ad' t',
-  matching_waits ad t1 ->
-  t1 --[e_init ad' t']--> t2 ->
-  matching_waits ad t2.
-Proof. solve_mwaits_preservation. Qed.
-
-Lemma mwaits_preservation_read : forall ad t1 t2 ad' t',
-  no_waits t' ->
-  (* --- *)
-  matching_waits ad t1 ->
-  t1 --[e_read ad' t']--> t2 ->
-  matching_waits ad t2.
-Proof. solve_mwaits_preservation. Qed.
-
-Lemma mwaits_preservation_write : forall ad t1 t2 ad' t',
-  matching_waits ad t1 ->
-  t1 --[e_write ad' t']--> t2 ->
-  matching_waits ad t2.
-Proof. solve_mwaits_preservation. Qed.
-
-Lemma mwaits_preservation_acq : forall ad t1 t2 ad' t' T,
-  no_waits t' ->
-  empty |-- t1 is T ->
-  (* --- *)
-  matching_waits ad t1 ->
-  t1 --[e_acq ad' t']--> t2 ->
-  matching_waits ad t2.
-Proof.
-  intros ad **. gendep ad. gendep T.
-  ind_tstep; intros; invc_typeof; repeat invc_mwaits; repeat constructor;
-  eauto using mwaits_from_nowaits, mwaits_subst.
-  rewrite <- empty_eq_safe_empty in *.
-  invc_typeof.
-  assert (~ (exists x' Tx' t', t = <{fn x' Tx' t'}>)). {
-    intros [? [? [? ?]]]. subst. invc_typeof.
-  }
-Qed.
-
-Lemma mwaits_preservation_rel : forall ad t1 t2 ad',
-  matching_waits ad t1 ->
-  t1 --[e_rel ad']--> t2 ->
-  matching_waits ad t2.
-Proof. solve_mwaits_preservation. Qed.
+From Elo Require Import NoWaits.
+From Elo Require Import ReservedWaits.
 
 (* ------------------------------------------------------------------------- *)
 (* valid-waits                                                               *)
 (* ------------------------------------------------------------------------- *)
 
+(* Enforces:
+    - x cannot be SELF in acquire statements.
+    - x cannot be SELF in function abstractions.
+    - the body of a function abstraction cannot have waits.
+*)
 Inductive valid_waits : tm -> Prop :=
-  | vwaits_unit   :                  valid_waits <{unit                     }>
-  | vwaits_nat    : forall n,        valid_waits <{nat n                    }>
-  | vwaits_plus   : forall t1 t2,    valid_waits t1 ->
-                                     valid_waits t2 ->
-                                     valid_waits <{t1 + t2                  }>
-  | vwaits_monus  : forall t1 t2,    valid_waits t1 ->
-                                     valid_waits t2 ->
-                                     valid_waits <{t1 - t2                  }>
-  | vwaits_seq    : forall t1 t2,    valid_waits t1 ->
-                                     valid_waits t2 ->
-                                     valid_waits <{t1; t2                   }>
-  | vwaits_if     : forall t1 t2 t3, valid_waits t1 ->
-                                     valid_waits t2 ->
-                                     valid_waits t3 ->
-                                     valid_waits <{if t1 then t2 else t3 end}>
-  | vwaits_while  : forall t1 t2,    valid_waits t1 ->
-                                     valid_waits t2 ->
-                                     valid_waits <{while t1 do t2 end       }>
-  | vwaits_var    : forall x,        valid_waits <{var x                    }>
-  | vwaits_fun    : forall x Tx t,   no_waits t     ->
-                                     valid_waits <{fn x Tx t                }>
-  | vwaits_call   : forall t1 t2,    valid_waits t1 ->
-                                     valid_waits t2 ->
-                                     valid_waits <{call t1 t2               }>
-  | vwaits_ref    : forall ad T,     valid_waits <{&ad : T                  }>
-  | vwaits_new    : forall t T,      valid_waits t  ->
-                                     valid_waits <{new t : T                }>
-  | vwaits_init   : forall ad t T,   valid_waits t  ->
-                                     valid_waits <{init ad t : T            }>
-  | vwaits_load   : forall t,        valid_waits t  ->
-                                     valid_waits <{*t                       }>
-  | vwaits_asg    : forall t1 t2,    valid_waits t1 ->
-                                     valid_waits t2 ->
-                                     valid_waits <{t1 := t2                 }>
-  | vwaits_acq    : forall t1 x t2,  valid_waits t1 ->
-                                     valid_waits <{acq t1 x t2              }>
-  | vwaits_cr     : forall ad t,     matching_waits ad t ->
-                                     valid_waits <{cr ad t                  }>
-  | vwaits_reacq  : forall ad',      valid_waits <{reacq ad'                }>
-  | vwaits_spawn  : forall t,        valid_waits t  ->
-                                     valid_waits <{spawn t                  }>
+  | vwaits_unit  :                  valid_waits <{unit                     }>
+  | vwaits_nat   : forall n,        valid_waits <{nat n                    }>
+  | vwaits_plus  : forall t1 t2,    valid_waits t1 ->
+                                    valid_waits t2 ->
+                                    valid_waits <{t1 + t2                  }>
+  | vwaits_monus : forall t1 t2,    valid_waits t1 ->
+                                    valid_waits t2 ->
+                                    valid_waits <{t1 - t2                  }>
+  | vwaits_seq   : forall t1 t2,    valid_waits t1 ->
+                                    valid_waits t2 ->
+                                    valid_waits <{t1; t2                   }>
+  | vwaits_if    : forall t1 t2 t3, valid_waits t1 ->
+                                    valid_waits t2 ->
+                                    valid_waits t3 ->
+                                    valid_waits <{if t1 then t2 else t3 end}>
+  | vwaits_while : forall t1 t2,    valid_waits t1 ->
+                                    valid_waits t2 ->
+                                    valid_waits <{while t1 do t2 end       }>
+  | vwaits_var   : forall x,        valid_waits <{var x                    }>
+  | vwaits_fun   : forall x Tx t,   x <> SELF      ->
+                                    no_waits    t  ->
+                                    valid_waits t  ->
+                                    valid_waits <{fn x Tx t                }>
+  | vwaits_call  : forall t1 t2,    valid_waits t1 ->
+                                    valid_waits t2 ->
+                                    valid_waits <{call t1 t2               }>
+  | vwaits_ref   : forall ad T,     valid_waits <{&ad : T                  }>
+  | vwaits_new   : forall t T,      valid_waits t  ->
+                                    valid_waits <{new t : T                }>
+  | vwaits_init  : forall ad t T,   valid_waits t  ->
+                                    valid_waits <{init ad t : T            }>
+  | vwaits_load  : forall t,        valid_waits t  ->
+                                    valid_waits <{*t                       }>
+  | vwaits_asg   : forall t1 t2,    valid_waits t1 ->
+                                    valid_waits t2 ->
+                                    valid_waits <{t1 := t2                 }>
+  | vwaits_acq   : forall t1 x t2,  x <> SELF        ->
+                                    valid_waits t1 ->
+                                    valid_waits t2 ->
+                                    valid_waits <{acq t1 x t2              }>
+  | vwaits_cr    : forall ad t,     valid_waits t  ->
+                                    valid_waits <{cr ad t                  }>
+  | vwaits_wait  : forall t,        valid_waits t  ->
+                                    valid_waits <{wait t                   }>
+  | vwaits_reacq : forall ad,       valid_waits <{reacq ad                 }>
+  | vwaits_spawn : forall t,        reserved_waits t ->
+                                    valid_waits t    ->
+                                    valid_waits <{spawn t                  }>
   .
 
 (* inversion --------------------------------------------------------------- *)
@@ -327,7 +74,7 @@ Local Ltac _vwaits tt :=
   | H : valid_waits <{_; _                  }> |- _ => tt H
   | H : valid_waits <{if _ then _ else _ end}> |- _ => tt H
   | H : valid_waits <{while _ do _ end      }> |- _ => tt H
-  | H : valid_waits <{var _                 }> |- _ => tt H
+  | H : valid_waits <{var _                 }> |- _ => clear H
   | H : valid_waits <{fn _ _ _              }> |- _ => tt H
   | H : valid_waits <{call _ _              }> |- _ => tt H
   | H : valid_waits <{&_ : _                }> |- _ => clear H
@@ -337,7 +84,7 @@ Local Ltac _vwaits tt :=
   | H : valid_waits <{_ := _                }> |- _ => tt H
   | H : valid_waits <{acq _ _ _             }> |- _ => tt H
   | H : valid_waits <{cr _ _                }> |- _ => tt H
-  | H : valid_waits <{wait _                }> |- _ => invc H
+  | H : valid_waits <{wait _                }> |- _ => tt H
   | H : valid_waits <{reacq _               }> |- _ => clear H
   | H : valid_waits <{spawn _               }> |- _ => tt H
   end.
@@ -347,83 +94,176 @@ Ltac invc_vwaits := _vwaits invc.
 
 (* lemmas ------------------------------------------------------------------ *)
 
-Lemma vwaits_from_nowaits : forall t,
-  no_waits t ->
-  valid_waits t.
+Lemma vwaits_init_term : forall t1 t2 ad' t',
+  valid_waits t1 ->
+  t1 --[e_init ad' t']--> t2 ->
+  valid_waits t'.
 Proof.
-  intros. induction t; invc_nowaits;
-  auto using mwaits_from_nowaits, valid_waits.
+  intros. ind_tstep; invc_vwaits; auto.
 Qed.
 
-Lemma nowaits_from_value2 : forall t,
+Lemma vwaits_write_term : forall t1 t2 ad' t',
+  valid_waits t1 ->
+  t1 --[e_write ad' t']--> t2 ->
+  valid_waits t'.
+Proof.
+  intros. ind_tstep; invc_vwaits; auto.
+Qed.
+
+Lemma rwaits_spawn_term : forall t1 t2 t',
+  valid_waits t1 ->
+  (* --- *)
+  t1 --[e_spawn t']--> t2 ->
+  reserved_waits t'.
+Proof.
+  intros. ind_tstep; invc_vwaits; auto.
+Qed.
+
+(* lemmas ------------------------------------------------------------------ *)
+
+Lemma nowaits_from_value : forall t,
   valid_waits t ->
   (* --- *)
-  value t ->
+  value t       ->
   no_waits t.
 Proof.
-  intros * ? Hval. invc Hval; auto using no_waits.
-  invc_vwaits. auto using no_waits.
+  intros * ? Hval. destruct Hval; invc_vwaits; auto using no_waits.
 Qed.
 
 (* preservation lemmas ----------------------------------------------------- *)
 
-Lemma vwaits_subst : forall t tx x,
+Lemma vwaits_subst : forall x tx t,
   value tx       ->
   (* --- *)
-  no_waits t     ->
+  valid_waits t  ->
   valid_waits tx ->
   valid_waits <{[x := tx] t}>.
-Proof.
-  eauto using vwaits_from_nowaits, nowaits_from_value2, nowaits_subst.
+Proof. 
+  intros. induction t; invc_vwaits;
+  simpl; repeat destruct _str_eq_dec;
+  auto using nowaits_from_value, nowaits_subst, rwaits_subst, valid_waits.
 Qed.
 
 (* preservation ------------------------------------------------------------ *)
 
-Local Ltac solve_vwaits_preservation L :=
-  intros; ind_tstep; repeat invc_vwaits; repeat constructor;
-  eauto using vwaits_subst, L.
+Local Ltac solve_vwaits_preservation :=
+  intros; ind_tstep; repeat invc_vwaits;
+  auto using vwaits_subst, valid_waits, value.
 
 Lemma vwaits_preservation_none : forall t1 t2,
   valid_waits t1 ->
   t1 --[e_none]--> t2 ->
   valid_waits t2.
-Proof. solve_vwaits_preservation mwaits_preservation_none. Qed.
+Proof. solve_vwaits_preservation. Qed.
 
 Lemma vwaits_preservation_alloc : forall t1 t2 ad' T',
   valid_waits t1 ->
   t1 --[e_alloc ad' T']--> t2 ->
   valid_waits t2.
-Proof. solve_vwaits_preservation mwaits_preservation_alloc. Qed.
+Proof. solve_vwaits_preservation. Qed.
 
-(* ------------------------------------------------------------------------- *)
+Lemma vwaits_preservation_init : forall t1 t2 ad' t',
+  valid_waits t1 ->
+  t1 --[e_init ad' t']--> t2 ->
+  valid_waits t2.
+Proof. solve_vwaits_preservation. Qed.
+
+Lemma vwaits_preservation_read : forall t1 t2 ad' t',
+  valid_waits t' ->
+  (* --- *)
+  valid_waits t1 ->
+  t1 --[e_read ad' t']--> t2 ->
+  valid_waits t2.
+Proof. solve_vwaits_preservation. Qed.
+
+Lemma vwaits_preservation_write : forall t1 t2 ad' t',
+  valid_waits t1 ->
+  t1 --[e_write ad' t']--> t2 ->
+  valid_waits t2.
+Proof. solve_vwaits_preservation. Qed.
+
+Lemma vwaits_preservation_acq : forall t1 t2 ad' t',
+  value t'       ->
+  valid_waits t' ->
+  (* --- *)
+  valid_waits t1 ->
+  t1 --[e_acq ad' t']--> t2 ->
+  valid_waits t2.
+Proof. solve_vwaits_preservation. Qed.
+
+Lemma vwaits_preservation_rel : forall t1 t2 ad',
+  valid_waits t1 ->
+  t1 --[e_rel ad']--> t2 ->
+  valid_waits t2.
+Proof. solve_vwaits_preservation. Qed.
+
+Lemma vwaits_preservation_wacq : forall t1 t2 ad',
+  valid_waits t1 ->
+  t1 --[e_wacq ad']--> t2 ->
+  valid_waits t2.
+Proof. solve_vwaits_preservation. Qed.
+
+Lemma vwaits_preservation_wrel : forall t1 t2 ad',
+  valid_waits t1 ->
+  t1 --[e_wrel ad']--> t2 ->
+  valid_waits t2.
+Proof. solve_vwaits_preservation. Qed.
+
+Lemma vwaits_preservation_spawn : forall t1 t2 t',
+  valid_waits t1 ->
+  t1 --[e_spawn t']--> t2 ->
+  valid_waits t2.
+Proof. solve_vwaits_preservation. Qed.
+
+Lemma vwaits_preservation_spawned : forall t1 t2 t',
+  valid_waits t1 ->
+  t1 --[e_spawn t']--> t2 ->
+  valid_waits t'.
+Proof. solve_vwaits_preservation. Qed.
+
+(* preservation ------------------------------------------------------------ *)
+
+Corollary vwaits_preservation_memory : forall m1 m2 ths1 ths2 tid e,
+  forall_threads ths1 valid_waits ->
+  forall_memory  m1   valid_waits ->
+  m1 \ ths1 ~~[tid, e]~~> m2 \ ths2 ->
+  forall_memory  m2   valid_waits.
+Proof.
+  intros. invc_cstep; try invc_mstep; trivial; intros ? ? ?;
+  upsilon; eauto using vwaits_init_term, vwaits_write_term.
+  omicron; upsilon; auto; eauto.
+Qed.
 
 Corollary vwaits_preservation_threads : forall m1 m2 ths1 ths2 tid e,
-  forall_memory  m1   valid_waits   ->
-  forall_threads ths1 valid_waits   ->
+  forall_memory  m1   value       ->
+  (* --- *)
+  forall_memory  m1   valid_waits ->
+  forall_threads ths1 valid_waits ->
   m1 \ ths1 ~~[tid, e]~~> m2 \ ths2 ->
   forall_threads ths2 valid_waits.
 Proof.
-  intros. invc_cstep; try invc_mstep; trivial.
-  - upsilon. eauto using vtm_preservation_none.
-  - upsilon. (* TODO: fix upsilon *)
-    intro tid'. sigma. upsilon. omicron.
-    + eauto using vtm_preservation_alloc.
-    + eauto using vtm_mem_add.
-  - upsilon; eauto using vtm_mem_set, vtm_preservation_init.
-  - upsilon. eauto using vtm_preservation_read.
-  - upsilon; eauto using vtm_mem_set, vtm_preservation_write.
-  - upsilon; eauto using vtm_mem_acq, vtm_preservation_acq.
-  - upsilon; eauto using vtm_mem_rel, vtm_preservation_rel.
-  - upsilon; eauto using vtm_mem_acq, vtm_preservation_wacq.
-  - upsilon; eauto using vtm_mem_rel, vtm_preservation_wrel.
-  - upsilon; eauto using vtm_preservation_spawn, vtm_preservation_spawned.
+  intros. invc_cstep; try invc_mstep; upsilon.
+  - eauto using vwaits_preservation_none. 
+  - eauto using vwaits_preservation_alloc. 
+  - eauto using vwaits_preservation_init.
+  - eauto using vwaits_preservation_read.
+  - eauto using vwaits_preservation_write.
+  - eauto using vwaits_preservation_acq.
+  - eauto using vwaits_preservation_rel.
+  - eauto using vwaits_preservation_wacq.
+  - eauto using vwaits_preservation_wrel.
+  - eauto using vwaits_preservation_spawn.
+  - eauto using vwaits_preservation_spawned.
 Qed.
 
 Theorem vwaits_preservation_cstep : forall m1 m2 ths1 ths2 tid e,
+  forall_memory  m1   value          ->
+  (* --- *)
   forall_program m1 ths1 valid_waits ->
-  m1 \ ths1 ~~[tid, e]~~> m2 \ ths2 ->
+  m1 \ ths1 ~~[tid, e]~~> m2 \ ths2  ->
   forall_program m2 ths2 valid_waits.
 Proof.
-  intros * [? ?] ?. split;
+  intros * ? [? ?] ?. split;
   eauto using vwaits_preservation_memory, vwaits_preservation_threads.
 Qed.
+
