Makefile
@@ -21,10 +21,15 @@ syntactic-properties:
 	$(COQC) NoRef.v
 	$(COQC) NoInit.v
 	$(COQC) NoCR.v
+	$(COQC) ValidTerm.v
+	# --- 
+	$(COQC) NoWaits.v
+	$(COQC) ReservedWaits.v
+	$(COQC) ValidWaits.v
+	$(COQC) ConsistentWaits.v
+	# --- 
 	$(COQC) HasVar.v
 	$(COQC) NoWRef.v
-	$(COQC) ValidWaits.v
-	$(COQC) ValidTerm.v
 	$(COQC) InheritanceNoInit.v
 	$(COQC) InheritanceNoCR.v
 	$(COQC) OneInit.v
